Added "arm_evalTheory" and "arm_evalLib" - this provides an IO free instruction set model with the memory as part of the state space.  Evaluation with this model is much simpler - some examples can be found in "run_arm_evalScript.sml".
The memory is updated with a new block substitution operator "::-".  A nifty
conversion SORT_BSUBST_CONV is used to simplify multiple applications of "::-".

examples/arm6/evaluate/arm_evalLib.sig
@@ -1,0 +1,23 @@
+signature arm_evalLib =
+sig
+   include Abbrev
+
+   val ARMe_CONV            : conv
+
+   val assemble1            : term -> Arbnum.num -> string -> term
+   val assemble             : term -> Arbnum.num -> string list -> term
+   val disassemble1         : term -> Arbnum.num -> string
+   val disassemble          : int -> term -> Arbnum.num -> string list
+
+   val set_registers        : term -> term -> term
+   val set_status_registers : term -> term -> term
+
+   val load_mem  : string -> int -> Arbnum.num -> term -> term
+   val save_mem  : string -> Arbnum.num -> Arbnum.num -> bool -> term -> unit
+   val list_mem  : int -> term -> Arbnum.num -> unit
+
+   val init      : term -> term -> term -> thm
+   val next      : thm -> thm
+   val eval      : int -> term -> term -> term -> thm list
+   val evaluate  : int -> term -> term -> term -> thm
+end
