examples/arm6/evaluate/arm_evalLib.sml
@@ -1,0 +1,259 @@
+(* ========================================================================= *)
+(* FILE          : arm_evalLib.sml                                           *)
+(* DESCRIPTION   : Code for evaluating the I/O free ARM specification        *)
+(*                                                                           *)
+(* AUTHOR        : (c) Anthony Fox, University of Cambridge                  *)
+(* DATE          : 2005                                                      *)
+(* ========================================================================= *)
+
+structure arm_evalLib :> arm_evalLib =
+struct
+
+(* interactive use:
+  app load ["Unix", "computeLib", "onestepTheory", "modelsLib",
+            "disassemblerLib", "arm_evalTheory"];
+*)
+
+open HolKernel boolLib bossLib;
+open Parse Q computeLib wordsSyntax rich_listTheory;
+open armTheory arm_evalTheory;
+
+(* ------------------------------------------------------------------------- *)
+
+val UNDEF_INST  = Arbnum.fromHexString "E6000010";
+val BINUTILS    = "/local/scratch/acjf3/gas/bin/arm-coff-";
+val AS_BIN      = BINUTILS ^ "as";
+val OBJCOPY_BIN = BINUTILS ^ "objcopy";
+
+(* ------------------------------------------------------------------------- *)
+(* Some conversions *)
+
+val SUC2NUM = CONV_RULE numLib.SUC_TO_NUMERAL_DEFN_CONV;
+
+fun add_rws f rws =
+let val cmp_set = f()
+    val _ = add_thms rws cmp_set
+in cmp_set end;
+
+fun arm_eval_compset () = let open simTheory in
+  add_rws modelsLib.arm_compset 
+    [ADDR30_def,SET_BYTE_def,BSUBST_EVAL,dimindex_30,finite_30,memop_case_def,
+     MEM_WRITE_BYTE_def,MEM_WRITE_WORD_def,MEM_WRITE_def,TRANSFERS_def,
+     SIMP_RULE (bool_ss++pred_setSimps.PRED_SET_ss) [] NEXT_ARMe_def]
+end;
+
+val ARMe_CONV = CBV_CONV (arm_eval_compset());
+val ARMe_RULE = CONV_RULE ARMe_CONV;
+
+val SORT_SUBST_CONV = let open simTheory
+  val compset = add_rws reduceLib.num_compset
+        [register_EQ_register,register2num_thm,psrs_EQ_psrs,psrs2num_thm,
+         SYM Sa_def,Sab_EQ,Sa_RULE4,Sb_RULE4,Sa_RULE_PSR,Sb_RULE_PSR,
+         combinTheory.o_THM]
+in
+  computeLib.CBV_CONV compset THENC PURE_REWRITE_CONV [Sa_def,Sb_def]
+end;
+
+val SORT_BSUBST_CONV = let open simTheory
+  val compset = add_rws wordsLib.words_compset
+        [dimindex_30,finite_30,LENGTH,SUC2NUM JOIN,SUC2NUM BUTFIRSTN,
+         APPEND,SUBST_BSUBST,BSa_RULE,BSb_RULE,GSYM BSa_def,combinTheory.o_THM]
+in
+  computeLib.CBV_CONV compset THENC PURE_REWRITE_CONV [BSa_def,BSb_def]
+end;
+
+val FOLD_SUBST_CONV = let open simTheory
+  val compset = add_rws wordsLib.words_compset
+      [SET_IFMODE_def,SET_NZCV_def,FOLDL,SUBST_EVAL,mode_num_def,mode_case_def,
+       register_EQ_register,register2num_thm,psrs_EQ_psrs,psrs2num_thm]
+in
+  computeLib.CBV_CONV compset THENC SORT_SUBST_CONV
+end;
+
+val SUBST_EQ_CONV = SIMP_CONV (srw_ss()) [SUBST_EQ2,simTheory.SUBST_EVAL];
+
+val rhsc = rhs o concl;
+
+fun printn s = print (s ^ "\n");
+
+(* ------------------------------------------------------------------------- *)
+(* Syntax *)
+
+fun mk_word30 n = mk_n2w(numSyntax.mk_numeral n,``:i30``);
+fun mk_word32 n = mk_n2w(numSyntax.mk_numeral n,``:i32``);
+
+fun eval_word t = (numSyntax.dest_numeral o rhsc o FOLD_SUBST_CONV o mk_w2n) t;
+
+val subst_tm  = prim_mk_const{Name = ":-",  Thy = "arm"};
+val bsubst_tm = prim_mk_const{Name = "::-", Thy = "sim"};
+
+fun mk_subst (a,b,m) =
+   list_mk_comb(inst[alpha |-> type_of a,beta |-> type_of b] subst_tm,[a,b,m])
+   handle HOL_ERR _ => raise ERR "mk_subst" "";
+
+fun mk_bsubst (a,b,m) =
+   list_mk_comb(inst[alpha |-> dim_of a,beta |-> listSyntax.eltype b]
+     bsubst_tm,[a,b,m])
+   handle HOL_ERR _ => raise ERR "mk_subst" "";
+
+val dest_subst  = dest_triop subst_tm  (ERR "dest_word_slice" "");
+val dest_bsubst = dest_triop bsubst_tm (ERR "dest_word_slice" "");
+
+fun dest_arm_eval t =
+  let val (h,l) = strip_comb t
+      val (h2, l2) = strip_comb (hd l)
+  in
+    if term_eq h ``ARM_EVAL`` andalso term_eq h2 ``ARM`` then
+      case (tl l,l2) of
+        ([m, u], [r, s]) => {mem = m, reg = r, psrs = s, undef = u}
+      | _ => raise ERR "dest_arm_eval" ""
+    else raise ERR "dest_arm_eval" ""
+  end
+  handle HOL_ERR _ => raise ERR "dest_arm_eval" "";
+
+(* ------------------------------------------------------------------------- *)
+(* Funtions for memory loading and saving *)
+
+local
+  fun bytes2num (b0,b1,b2,b3) =
+    let open Arbnum
+        val byte2num = fromInt o Char.ord o Byte.byteToChar
+    in
+      (byte2num b0) * (fromInt 16777216) + (byte2num b1) * (fromInt 65536) +
+      (byte2num b2) * (fromInt 256) + byte2num b3
+    end
+
+  fun read_word (v,i) =
+    let val l = Word8Vector.length v
+        fun f i = if i < l then Word8Vector.sub(v,i) else 0wx0
+    in
+      mk_word32 (bytes2num (f i, f (i + 1), f (i + 2), f (i + 3)))
+      (* could change order to do little-endian *)
+    end
+in
+  fun load_mem fname skip top_addr m =
+    let open BinIO
+        val istr = openIn fname
+        val data = inputAll istr
+        val _ = closeIn istr
+        val lines = (Word8Vector.length data - skip) div 4
+        val l = List.tabulate(lines, fn i => read_word (data,4 * i + skip))
+        val lterm = listSyntax.mk_list(l,``:word32``)
+    in
+      rhsc (SORT_BSUBST_CONV (mk_bsubst(mk_word30 top_addr,lterm,m)))
+    end
+end;
+
+fun mem_read m a = (eval_word o rhsc o ARMe_CONV) (mk_comb(m,mk_word30 a));
+
+fun save_mem fname start finish le m = let open BinIO Arbnum
+    fun bits  h l n = (n mod pow(two,plus1 h)) div (pow(two,l))
+    val ostr = openOut fname
+    val num2byte = Word8.fromInt o Arbnum.toInt;
+    fun num2bytes w =
+          map (fn (i,j) => num2byte (bits (fromInt i) (fromInt j) w))
+              ((if le then rev else I) [(31,24),(23,16),(15,8),(7,0)])
+    fun save_word i = map (fn b => output1(ostr,b)) (num2bytes (mem_read m i))
+    fun recurse i =
+          if Arbnum.<=(i,finish) then recurse (save_word i; Arbnum.plus1 i)
+          else closeOut ostr
+in
+  recurse start
+end;
+
+(* ------------------------------------------------------------------------- *)
+
+(* -----------
+ A suitable ARM code binary can be generated using GNU's binutils:
+
+   arm-coff-as -EB assembler.s
+   arm-coff-objcopy -S -j .text a.out code
+
+ Then a skip of 60 is needed to pass over the header of the COFF binary
+   ----------- *)
+
+fun assemble m a s =
+  let val as_ex  = Unix.execute(AS_BIN,["-EB","-aln"])
+      val (inp,out) = Unix.streamsOf as_ex
+      val _ = TextIO.output(out,String.concat (map (fn t => t ^ "\n") s))
+      val _ = TextIO.closeOut out
+      val err = TextIO.inputAll inp
+      val _ = TextIO.closeIn inp
+      val args = ["-S","-j",".text","a.out","a.out"]
+      val objcopy_ex = Unix.execute(OBJCOPY_BIN, args)
+      val _ = Unix.reap objcopy_ex
+  in
+    load_mem "a.out" 60 a m handle _ => (printn err; m)
+  end;
+
+fun assemble1 m a s =
+   let val x = if s = "" then UNDEF_INST else Arbnum.fromHexString s in
+      mk_subst(mk_word30 a,mk_word32 x,m)
+   end handle _ => assemble m a [s];
+
+fun disassemble1 m a = disassemblerLib.opcode_string (mem_read m a)
+
+local
+  fun recurse n m a l =
+    if n = 0 then l
+    else recurse (n - 1) m (Arbnum.plus1 a) (disassemble1 m a :: l)
+in
+  fun disassemble n m a = rev (recurse n m a [])
+end;
+
+fun list_mem n m a =
+  let val l = disassemble n m a in
+    (print o String.concat o (map (fn t => t ^ "\n"))) l
+  end;
+
+(* ------------------------------------------------------------------------- *)
+(* Set the general purpose and program status registers *)
+
+val foldl_tm = ``FOLDL (\m (r,v). if v = m r then m else (r :- v) m) x y``;
+
+fun set_registers reg rvs  =
+ (rhsc o FOLD_SUBST_CONV o
+  subst [``x:reg`` |-> reg, ``y:(register # word32) list`` |-> rvs] o
+  inst [alpha |-> ``:register``, beta |-> ``:word32``]) foldl_tm;
+
+fun set_status_registers psr rvs  = (rhsc o 
+  (FOLD_SUBST_CONV
+     THENC PURE_ONCE_REWRITE_CONV [SPEC `n2w n` simTheory.PSR_CONS]
+     THENC ARMe_CONV) o
+  subst [``x:psr`` |-> psr, ``y:(psrs # word32) list`` |-> rvs] o
+  inst [alpha |-> ``:psrs``, beta |-> ``:word32``]) foldl_tm;
+
+(* ------------------------------------------------------------------------- *)
+(* Running the model *)
+
+fun init m r s =
+   (PURE_ONCE_REWRITE_CONV [CONJUNCT1 STATE_ARMe_def] o
+    subst [``mem:mem`` |-> m, ``reg:reg`` |-> r, ``psr:psr`` |-> s])
+   ``STATE_ARMe 0 (ARM_EVAL (ARM reg psr) mem F)``;
+
+fun next t =
+  let val t1 = rhsc t
+      val t2 = ((ARMe_CONV THENC ONCE_DEPTH_CONV SORT_BSUBST_CONV
+                   THENC ONCE_DEPTH_CONV SORT_SUBST_CONV
+                   THENC SUBST_EQ_CONV) o
+                 subst [``s:state_arme`` |-> t1]) ``NEXT_ARMe s``
+      val STATE_ARMe_NEXT = MATCH_MP onestepTheory.IMAP_NEXT STATE_ARMe_THM;
+  in
+     numLib.REDUCE_RULE (MATCH_MP STATE_ARMe_NEXT (CONJ t t2))
+  end;
+
+fun done t = term_eq T (#undef (dest_arm_eval (rhsc t)));
+
+fun state n [] = []
+  | state n (l as (t::ts)) =
+      if n = 0 then l
+      else let val nl = (time next t) :: l in
+        if done t then nl else state (n - 1) nl
+      end;
+
+fun eval n m r s = state n [init m r s];
+fun evaluate n m r s = hd (eval n m r s);
+
+(* ------------------------------------------------------------------------- *)
+
+end
