examples/arm6/evaluate/disassemblerLib.sig
@@ -1,14 +1,10 @@
 signature  disassemblerLib =
 sig
   val opcode_string : Arbnum.num -> string
-  val psr_string : Arbnum.num -> string
-  val is_coproc : Arbnum.num -> bool
-  val pp_word_psr : unit -> unit
-  val pp_word_pipe : unit -> unit
-  val pp_word_arm_ex : unit -> unit
-  val pp_word_arm : unit -> unit
-  val npp_word_psr : unit -> unit
-  val npp_word_pipe : unit -> unit
-  val npp_word_arm_ex : unit -> unit
-  val npp_word_arm : unit -> unit
+  val psr_string    : Arbnum.num -> string
+  val is_coproc     : Arbnum.num -> bool
+  val pp_arm        : unit -> unit
+  val pp_arm6       : unit -> unit
+  val npp_arm       : unit -> unit
+  val npp_arm6      : unit -> unit
 end
