examples/arm6/evaluate/modelsLib.sml
@@ -23,12 +23,39 @@ fun NUMERAL_ONLY_RULE n x =
 
 val EXTRACT_RULE = SIMP_RULE std_ss [w2w_def,word_extract_def];
 
+val common_thms =
+  [FST,SND,SUC_RULE EL,HD,TL,MAP,FILTER,LENGTH,ZIP,FOLDL,
+   SUC_RULE rich_listTheory.GENLIST,rich_listTheory.SNOC,
+   SUC_RULE rich_listTheory.FIRSTN,combinTheory.K_THM,
+   register_EQ_register,num2register_thm,register2num_thm,
+   mode_EQ_mode,mode2num_thm,mode_case_def,
+   psrs_EQ_psrs,psrs2num_thm,
+   iclass_EQ_iclass,iclass2num_thm,
+   exception_EQ_exception,exception2num_thm,exception_case_def,
+   num2exception_thm,exception2mode_def,
+   num2condition_thm,condition2num_thm,condition_case_def,
+   interrupts_case_def,
+   SUBST_EVAL,
+
+   SET_NZC_def,NZCV_def,USER_def,INC_IS,INC_IS_def,mode_num_def,
+   EXTRACT_RULE DECODE_IFMODE_SET_NZCV,DECODE_NZCV_SET_NZCV,
+   EXTRACT_RULE DECODE_IFMODE_SET_IFMODE,DECODE_NZCV_SET_IFMODE,
+   SET_NZCV_IDEM,SET_IFMODE_IDEM,SET_IFMODE_NZCV_SWP,
+   DECODE_PSR_def,DECODE_MODE_def,DECODE_PSR_THM,
+   CPSR_READ_def,CPSR_WRITE_def,SPSR_READ_def,SPSR_WRITE_def,
+   CPSR_WRITE_n2w,SPSR_WRITE_n2w,mode_reg2num_def,mode2psr_def,
+   REG_READ_def,REG_WRITE_def,INC_PC_def,FETCH_PC_def,REG_READ6_def,
+   REG_WRITE_PSR,REG_WRITE_PSR2,word_modify_PSR,word_modify_PSR2,
+   ALU_arith_def,ALU_arith_neg_def,ALU_logic_def,SUB_def,ADD_def,
+   AND_def,EOR_def,ORR_def,ALU_def,
+   LSL_def,LSR_def,ASR_def,ROR_def,RRX2_def,
+   CONDITION_PASSED_def,CONDITION_PASSED2_def,
+   NUMERAL_ONLY_RULE `n` DECODE_INST_THM,MLA_MUL_DUR_n2w];
+
 fun arm_compset () =
   let val compset = wordsLib.words_compset ()
-      val thms =
-       [FST,SND,SUC_RULE EL,HD,TL,MAP,FILTER,LENGTH,ZIP,FOLDL,
-        SUC_RULE rich_listTheory.GENLIST,rich_listTheory.SNOC,
-        SUC_RULE rich_listTheory.FIRSTN,combinTheory.K_THM,
+      val thms = common_thms @
+       [ZIP,FOLDL,
         state_inp_accessors, state_inp_updates_eq_literal,
         state_inp_accfupds, state_inp_fupdfupds, state_inp_literal_11,
         state_inp_fupdfupds_comp, state_inp_fupdcanon,
@@ -37,49 +64,29 @@ fun arm_compset () =
         state_out_accfupds, state_out_fupdfupds, state_out_literal_11,
         state_out_fupdfupds_comp, state_out_fupdcanon,
         state_out_fupdcanon_comp,
-        register_EQ_register,num2register_thm,register2num_thm,
-        mode_EQ_mode,mode2num_thm,
-        psrs_EQ_psrs,psrs2num_thm,
-        iclass_EQ_iclass,iclass2num_thm,
-        exception_EQ_exception,num2exception_thm,
-        exception2num_thm,exception2mode_def,
-        num2condition_thm,condition2num_thm,
-        mode_case_def,condition_case_def,
-        exception_case_def,interrupts_case_def,
-        SYM Sa_def,Sa_EVAL,Sb_EVAL,Sab_EQ,
-        Sa_RULE4,Sb_RULE4,
-        Sa_RULE_PSR,Sb_RULE_PSR,
+
         DECODE_BRANCH_THM,DECODE_DATAP_THM,DECODE_MRS_THM,
         DECODE_MSR_THM,DECODE_LDR_STR_THM,DECODE_SWP_THM,
         DECODE_LDM_STM_THM,DECODE_MLA_MUL_THM,DECODE_LDC_STC_THM,
-        CARRY_def,USER_def,mode_num_def,SET_NZC_def,NZCV_def,
-        EXTRACT_RULE DECODE_IFMODE_SET_NZCV,DECODE_NZCV_SET_NZCV,
-        EXTRACT_RULE DECODE_IFMODE_SET_IFMODE,DECODE_NZCV_SET_IFMODE,
-        SET_NZCV_IDEM,SET_IFMODE_IDEM,SET_IFMODE_NZCV_SWP,
-        DECODE_PSR_def,DECODE_PSR_THM,DECODE_MODE_def,
-        CPSR_READ_def,CPSR_WRITE_def,SPSR_READ_def,SPSR_WRITE_def,
-        mode2psr_def,mode_reg2num_def,
-        REG_READ_def,REG_WRITE_def,FETCH_PC_def,INC_PC_def,BW_READ_def,
+
+        CARRY_def,BW_READ_def,
         SHIFT_IMMEDIATE2_def,SHIFT_REGISTER2_def,
         SHIFT_IMMEDIATE_THM,SHIFT_REGISTER_THM,IMMEDIATE_def,
-        ALU_multiply_def,ALU_arith_def,ALU_arith_neg_def,ALU_logic_def,
-        SUB_def,ADD_def,AND_def,EOR_def,ORR_def,
-        LSL_def,LSR_def,ASR_def,ROR_def,RRX2_def,
-        ALU_def,ARITHMETIC_def,TEST_OR_COMP_def,UP_DOWN_def,
+        ALU_multiply_def,ARITHMETIC_def,TEST_OR_COMP_def,UP_DOWN_def,
         ADDR_MODE1_def,ADDR_MODE2_def,ADDR_MODE4_def,ADDR_MODE5_def,
+        REGISTER_LIST_THM,ADDRESS_LIST_def,FIRST_ADDRESS_def,WB_ADDRESS_def,
+        LDM_LIST_def,STM_LIST_def,BORROW2_def,MSHIFT2_def,MLA_MUL_CARRY_def,
+
         EXCEPTION_def,BRANCH_def,DATA_PROCESSING_def,MRS_def,LDR_STR_def,
         MLA_MUL_def,SWP_def,MRC_def,MCR_OUT_def,MSR_def,LDM_STM_def,LDC_STC_def,
-        REGISTER_LIST_THM,ADDRESS_LIST_def,LDM_LIST_def,STM_LIST_def,
-        BORROW2_def,MSHIFT2_def,MLA_MUL_CARRY_def,MLA_MUL_DUR_n2w,
-        NUMERAL_ONLY_RULE `n` DECODE_INST_THM,EXEC_INST_def,
-        CONDITION_PASSED_def,CONDITION_PASSED2_def,
+
         SIMP_RULE (std_ss++pred_setSimps.PRED_SET_ss) []
           interrupt2exception_def,
         IS_Dabort_def,IS_Reset_def,PROJ_Dabort_def,PROJ_Reset_def,
         THE_DEF,IS_SOME_DEF,IS_NONE_EQ_NONE,NOT_IS_SOME_EQ_NONE,
         option_case_ID,option_case_SOME_ID,
         option_case_def,SOME_11,NOT_SOME_NONE,PROJ_IF_FLAGS_def,
-        NEXT_ARM_def,OUT_ARM_def]
+        EXEC_INST_def,NEXT_ARM_def,OUT_ARM_def]
        val _ = add_thms thms compset
 in
   compset
@@ -87,21 +94,9 @@ end;
 
 fun arm6_compset () =
   let val compset = wordsLib.words_compset ()
-      val thms =
-       [SUC_RULE EL,HD,TL,MAP,FILTER,LENGTH,
-        SUC_RULE rich_listTheory.GENLIST,rich_listTheory.SNOC,
-        SIMP_RULE std_ss [] REGISTER_LIST_def,
-        SUC_RULE sum_numTheory.SUM_def,
-        exception2mode_def,
-        register_EQ_register,mode_EQ_mode,psrs_EQ_psrs,
-        iclass_EQ_iclass,iseq_EQ_iseq,
-        register2num_thm,mode2num_thm,psrs2num_thm,iclass2num_thm,
-        iseq2num_thm, exception2num_thm,
-        num2register_thm, num2condition_thm, num2exception_thm, num2iseq_thm,
-        mode_case_def, condition_case_def, exception_case_def,
-        SYM Sa_def,Sa_EVAL,Sb_EVAL,Sab_EQ,
-        Sa_RULE4,Sb_RULE4,Sa_RULE_PSR,Sb_RULE_PSR,
-        FST,SND,INC_IS,
+      val thms = common_thms @
+       [SIMP_RULE std_ss [] REGISTER_LIST_def,SUC_RULE sum_numTheory.SUM_def,
+        iseq_EQ_iseq, iseq2num_thm, num2iseq_thm,
 
         CLEARBIT_def,NUMERAL_LEASTBIT16,
         NMREQ_def,PCWA_def,
@@ -115,28 +110,12 @@ fun arm6_compset () =
         ABORTINST_def,DATAABT_def,IC_def,IS_def,COPROC1_def,DATAABT1_def,
         FIQACT_def,IRQACT_def,PCCHANGE_def,RESETLATCH_def,RESETSTART_def,
         INTSEQ_def,NEWINST_def,PIPEALL_def,PIPEBLL_def,PIPECWRITE_def,
-        NXTIC_def,INC_IS_def,NXTIS_def,PIPEAWRITE_def,PIPEBWRITE_def,
+        NXTIC_def,NXTIS_def,PIPEAWRITE_def,PIPEBWRITE_def,
         PIPESTATAWRITE_def,PIPESTATBWRITE_def,PIPESTATIREGWRITE_def,
         PIPEAVAL_def,IREGVAL_def,PIPEAABT_def,
         IREGABT2_def,AREGN1_def,ENDINST_def,
 
-        SET_NZC_def,NZCV_def,USER_def,mode_num_def,
-        EXTRACT_RULE DECODE_IFMODE_SET_NZCV,DECODE_NZCV_SET_NZCV,
-        EXTRACT_RULE DECODE_IFMODE_SET_IFMODE,DECODE_NZCV_SET_IFMODE,
-        SET_NZCV_IDEM,SET_IFMODE_IDEM,SET_IFMODE_NZCV_SWP,
-        DECODE_PSR_def,DECODE_MODE_def,DECODE_PSR_THM,
-        CPSR_READ_def,CPSR_WRITE_def,
-        SPSR_READ_def,SPSR_WRITE_def,
-        mode_reg2num_def,mode2psr_def,
-        REG_READ_def,REG_WRITE_def,INC_PC_def,FETCH_PC_def,REG_READ6_def,
-        ALU_arith_def,ALU_arith_neg_def,ALU_logic_def,SUB_def,ADD_def,
-        AND_def,EOR_def,ORR_def,ALU_def,
-        LSL_def,LSR_def,ASR_def,ROR_def,RRX2_def,
-
-        CONDITION_PASSED_def,CONDITION_PASSED2_def,
-        NUMERAL_ONLY_RULE `n` DECODE_INST_THM,
-        PROJ_NRESET_def,PROJ_ABORT_def,IS_RESET_def,IS_ABORT_def,
-        MLA_MUL_DUR_n2w,DUR_IC_def,
+        PROJ_NRESET_def,PROJ_ABORT_def,IS_RESET_def,IS_ABORT_def,DUR_IC_def,
         INIT_ARM6_def,NEXT_ARM6_def,OUT_ARM6_def,CONJUNCT1 STATE_ARM6_def]
       val _ = add_thms thms compset
 in
