examples/arm6/evaluate/run_arm_evalLib.sml
@@ -1,0 +1,149 @@
+(* ========================================================================= *)
+(* FILE          : run_arm_evalLib.sml                                       *)
+(* DESCRIPTION   : Examples using arm_evalLib                                *)
+(*                                                                           *)
+(* AUTHOR        : (c) Anthony Fox, University of Cambridge                  *)
+(* DATE          : 2005                                                      *)
+(* ========================================================================= *)
+
+(* interactive use:
+  load "arm_evalLib";
+*)
+
+open HolKernel boolLib bossLib;
+open arm_evalLib;
+
+(* ------------------------------------------------------------------------- *)
+
+val zero = Arbnum.zero;
+val max = valOf Int.maxInt;
+
+(* Assemble a rudimentary exception handler *)
+
+val mem = assemble ``\x:word30. 0xE6000010w:word32`` zero
+  ["movs pc, #32",
+   "label: b label",
+   "movs pc, r14",
+   "subs pc, r14, #4",
+   "subs pc, r14, #8",
+   "movs pc, r14",
+   "subs pc, r14, #4",
+   "subs pc, r14, #4"];
+
+(*
+val EXC_HANDLER = "handler";
+val _ = save_mem EXC_HANDLER zero (Arbnum.fromInt 7) false mem;
+*)
+
+(* Initial general purpose register values *)
+
+val reg = set_registers ``(\x. 0w):reg``
+ ``[(r0,0w);  (r1,0w);  (r2,0w);  (r3,0w);
+    (r4,0w);  (r5,0w);  (r6,0w);  (r7,0w);
+    (r8,0w);  (r9,0w);  (r10,0w); (r11,0w);
+    (r12,0w); (r13,0w); (r14,0w); (r15,0w);
+    (r8_fiq,0w); (r9_fiq,0w); (r10_fiq,0w); (r11_fiq,0w);
+    (r12_fiq,0w); (r13_fiq,0w); (r14_fiq,0w);
+    (r13_irq,0w); (r14_irq,0w);
+    (r13_svc,0w); (r14_svc,0w);
+    (r13_abt,0w); (r14_abt,0w);
+    (r13_und,0w); (r14_und,0w)]: (register # word32) list``;
+
+(* Initial program status register values *)
+
+val psr = set_status_registers
+ ``(\x. SET_NZCV (F,F,F,F) (SET_IFMODE F F usr 0w)):psr``
+ ``[(CPSR,SET_NZCV (F,F,F,F) (SET_IFMODE F F svc 0w))]: (psrs # word32) list``;
+
+(* ------------------------------------------------------------------------- *)
+
+(* Testing/Examples *)
+
+val prog1 = assemble1 mem (Arbnum.fromInt 8) "mov r0, #1";
+
+val res1 = evaluate max prog1 reg psr;
+
+val prog2 = assemble mem (Arbnum.fromInt 8)
+  ["mov r0, #12",
+   "mov r1, #10",
+   "eor r2, r0, r1",
+   "and r3, r0, r1",
+   "orr r4, r0, r1",
+   "bic r5, r0, r1"];
+
+val res2 = evaluate max prog2 reg psr;
+
+val prog3 = assemble mem (Arbnum.fromInt 8)
+  [       "mov r0, #10",
+   "label: add r0, r0, #1",
+          "cmp r0, #12",
+          "bne label"];
+
+val res3 = evaluate max prog3 reg psr;
+
+val prog4 = assemble mem (Arbnum.fromInt 8)
+  ["mov r0, #0xF",
+   "mov r1, #4",
+   "mvn r2, r0, lsl r1",
+   "add r3, r3, r0, lsl #8",
+   "mov r4, r0, ror #4",
+   "mov r5, r4, lsr #4",
+   "mov r6, r4, asr #16"];
+
+val res4 = evaluate max prog4 reg psr;
+
+val prog5 = assemble mem (Arbnum.fromInt 8)
+  ["mov r0, #0xF",
+   "mov r1, #4",
+   "mvn r2, r0, lsl r1",
+   "add r3, r3, r0, lsl #8",
+   "mov r4, r0, ror #4",
+   "mov r5, r4, lsr #4",
+   "mov r6, r4, asr #16"];
+
+val res5 = evaluate max prog5 reg psr;
+
+val prog6 = assemble mem (Arbnum.fromInt 8)
+  ["mov r0, #8",
+   "mov r1, #12",
+   "mul r2, r0, r1",
+   "mla r3, r2, r1, r2"];
+
+val res6 = evaluate max prog6 reg psr;
+
+val prog7 = assemble mem (Arbnum.fromInt 8)
+  ["mov  r0, #0xFF",
+   "mul  r0, r0, r0",
+   "str  r0, [r0], #4",
+   "strb r0, [r0]",
+   "ldr  r1, [r0]",
+   "ldrb r2, [r3]"];
+
+val res7 = evaluate max prog7 reg psr;
+
+val prog8 = assemble mem (Arbnum.fromInt 8)
+  ["ldmia r0, {r1-r10}",
+   "stmdb r1, {r1-r10}"];
+
+val res8 = evaluate max prog8 reg psr;
+
+val prog9 = assemble mem (Arbnum.fromInt 8)
+  ["mov  r0, #77",
+   "mov  r1, #88",
+   "mov  r2, #0xF00",
+   "swp  r0, r1, [r2]",
+   "swpb r3, r1, [r0]"];
+
+val res9 = evaluate max prog9 reg psr;
+
+val prog10 = assemble ``\x:word30. 0xE6000010w:word32`` zero
+  ["mrs r0, CPSR",
+   "mrs r1, SPSR",
+   "mov r2, #0xF0000000",
+   "orr r2, r2, #0x12",
+   "msr CPSR, r2",
+   "msr SPSR_c, r2"];
+
+val res10 = evaluate 6 prog10 reg psr;
+
+(* ------------------------------------------------------------------------- *)
