examples/arm6/evaluate/arm_evalScript.sml
@@ -1,0 +1,109 @@
+(* ========================================================================= *)
+(* FILE          : arm_evalScript.sml                                        *)
+(* DESCRIPTION   : I/O and exception free model of the ARM ISA               *)
+(*                                                                           *)
+(* AUTHORS       : (c) Anthony Fox, University of Cambridge                  *)
+(* DATE          : 2005                                                      *)
+(* ========================================================================= *)
+
+(* interactive use:
+  app load ["wordsLib", "armTheory", "simTheory"];
+*)
+
+open HolKernel boolLib Parse bossLib;
+open Q wordsLib onestepTheory armTheory;
+
+val _ = new_theory "arm_eval";
+
+(* ------------------------------------------------------------------------- *)
+(* The State Space --------------------------------------------------------- *)
+(* ------------------------------------------------------------------------- *)
+
+val _ = mk_word_type 30;
+
+val _ = type_abbrev("mem", ``:word30->word32``);
+
+val _ = Hol_datatype `state_arme = ARM_EVAL of state_arm=>mem=>bool`;
+
+(* ------------------------------------------------------------------------- *)
+
+val ADDR30_def = Define `ADDR30 (addr:word32) = (31 >< 2) addr:word30`;
+
+val SET_BYTE_def = Define`
+  SET_BYTE (oareg:word2) (b:word8) (w:word32) =
+    word_modify (\i x.
+                  (i < 8) /\ (if oareg = 0w then b %% i else x) \/
+       (8 <= i /\ i < 16) /\ (if oareg = 1w then b %% (i - 8) else x) \/
+      (16 <= i /\ i < 24) /\ (if oareg = 2w then b %% (i - 16) else x) \/
+      (24 <= i /\ i < 32) /\ (if oareg = 3w then b %% (i - 24) else x)) w`;
+
+val MEM_WRITE_BYTE_def = Define`
+  MEM_WRITE_BYTE (mem:mem) (word:word32) addr =
+    let addr30 = ADDR30 addr in
+      (addr30 :- SET_BYTE ((1 >< 0) addr) ((7 >< 0) word) (mem addr30)) mem`;
+
+val MEM_WRITE_WORD_def = Define`
+  MEM_WRITE_WORD (mem:mem) word addr = (ADDR30 addr :- word) mem`;
+
+val MEM_WRITE_def = Define`
+  MEM_WRITE b = if b then MEM_WRITE_BYTE else MEM_WRITE_WORD`;
+
+val TRANSFERS_def = Define`
+  (TRANSFERS mem data [] = (mem,data)) /\
+  (TRANSFERS mem data (r::rs) =
+   case r of
+      MemRead addr -> TRANSFERS mem (SNOC (mem (ADDR30 addr)) data) rs
+   || MemWrite B addr word -> TRANSFERS (MEM_WRITE B mem word addr) data rs
+   || _ -> TRANSFERS mem data rs)`;
+
+val NEXT_ARMe_def = Define`
+  NEXT_ARMe (ARM_EVAL (ARM reg psr) mem undef) =
+    let pc = FETCH_PC reg in
+    let ireg = mem (ADDR30 pc) in
+    let s = ARM_EX (ARM reg psr) ireg (if undef then undefined else software) in
+    let mrqs = OUT_ARM s in
+    let (str_mem,data) = TRANSFERS mem [] mrqs in
+    let ns = EXEC_INST s NONE data T
+    in
+      ARM_EVAL ns str_mem (DECODE_INST ireg IN {cdp_und; mrc; mcr; stc; ldc})`;
+
+val STATE_ARMe_def = Define`
+  (STATE_ARMe 0 s = s) /\
+  (STATE_ARMe (SUC t) s = NEXT_ARMe (STATE_ARMe t s))`;
+
+(* ------------------------------------------------------------------------- *)
+
+infix \\ << >>
+
+val op \\ = op THEN;
+val op << = op THENL;
+val op >> = op THEN1;
+
+val STATE_ARMe_THM = store_thm("STATE_ARMe_THM",
+  `IMAP STATE_ARMe I NEXT_ARMe`,
+  RW_TAC (std_ss++boolSimps.LET_ss)
+    [STATE_ARMe_def,IMAP_def,combinTheory.I_THM]);
+
+val Sa_RULE_WORD = store_thm("Sa_RULE_WORD",
+  `!m a b d e. Sa a e (Sa b d m) =
+     if a <+ b then
+       Sb b d (Sa a e m)
+     else
+       Sb a e (Sa b d m)`,
+  METIS_TAC [simTheory.Sa_def,simTheory.Sb_def,SUBST_COMMUTES]);
+
+val Sb_RULE_WORD = store_thm("Sb_RULE_WORD",
+  `!m a b d e. Sa a e (Sb b d m) =
+     if a <+ b then
+       Sb b d (Sa a e m)
+     else
+       Sb a e (Sb b d m)`,
+  METIS_TAC [simTheory.Sa_def,simTheory.Sb_def,SUBST_COMMUTES]);
+
+val SUBST_EQ2 = store_thm("SUBST_EQ2",
+  `!m a v. (m a = v) ==> ((a :- v) m = m)`,
+  REPEAT STRIP_TAC \\ REWRITE_TAC [FUN_EQ_THM] \\ RW_TAC std_ss [SUBST_def]);
+
+(* ------------------------------------------------------------------------- *)
+
+val _ = export_theory();
